Source/Concurrency/LinearRewriter.cs
@@ -24,6 +24,9 @@ public class LinearRewriter
 
   public static void Rewrite(CivlTypeChecker civlTypeChecker, Implementation impl)
   {
+    if (IsPrimitive(impl)) {
+      return;
+    }
     var linearRewriter = new LinearRewriter(civlTypeChecker);
     impl.Blocks.ForEach(block => block.Cmds = linearRewriter.RewriteCmdSeq(block.Cmds));
   }
@@ -69,28 +72,14 @@ public class LinearRewriter
   {
     switch (Monomorphizer.GetOriginalDecl(callCmd.Proc).Name)
     {
-      case "Ref_Alloc":
-        return RewriteRefAlloc(callCmd);
-      case "Lheap_Empty":
-        return RewriteLheapEmpty(callCmd);
-      case "Lheap_Alloc":
-        return RewriteLheapAlloc(callCmd);
-      case "Lheap_Free":
-        return RewriteLheapFree(callCmd);
-      case "Lheap_Get":
-        return RewriteLheapGet(callCmd);
-      case "Lheap_Put":
-        return RewriteLheapPut(callCmd);
+      case "Loc_New":
       case "Lmap_Empty":
-        return RewriteLmapEmpty(callCmd);
       case "Lmap_Alloc":
-        return RewriteLmapAlloc(callCmd);
+      case "Lmap_Create":
       case "Lmap_Free":
-        return RewriteLmapFree(callCmd);
-      case "Lmap_Get":
-        return RewriteLmapGet(callCmd);
-      case "Lmap_Put":
-        return RewriteLmapPut(callCmd);
+      case "Lmap_Move":
+      case "Lmap_Assume":
+        return new List<Cmd>{callCmd};
       case "Lset_Empty":
         return RewriteLsetEmpty(callCmd);
       case "Lset_Split":
@@ -148,14 +137,9 @@ public class LinearRewriter
     return monomorphizer.InstantiateFunction("MapIte",new Dictionary<string, Type>() { { "T", domain }, { "U", range } });
   }
 
-  private Function LheapContains(Type type)
+  private Function MapContains(Type keyType, Type valueType)
   {
-    return monomorphizer.InstantiateFunction("Lheap_Contains",new Dictionary<string, Type>() { { "V", type } });
-  }
-
-  private Function LheapDeref(Type type)
-  {
-    return monomorphizer.InstantiateFunction("Lheap_Deref",new Dictionary<string, Type>() { { "V", type } });
+    return monomorphizer.InstantiateFunction("Map_Contains",new Dictionary<string, Type>() { {"T", keyType}, { "U", valueType } });
   }
 
   private Function LsetContains(Type type)
@@ -179,252 +163,9 @@ public class LinearRewriter
     return ExprHelper.FunctionCall(defaultFunc);
   }
 
-  private List<Cmd> RewriteRefAlloc(CallCmd callCmd)
-  {
-    GetRelevantInfo(callCmd, out Type type, out Type refType, out Function lheapConstructor,
-      out Function lsetConstructor, out Function lvalConstructor);
-    var instantiation = monomorphizer.GetTypeInstantiation(callCmd.Proc);
-    var nilFunc = monomorphizer.InstantiateFunction("Nil", instantiation);
-
-    var cmdSeq = new List<Cmd>();
-    var k = callCmd.Outs[0];
-
-    cmdSeq.Add(CmdHelper.HavocCmd(k));
-    cmdSeq.Add(CmdHelper.AssumeCmd(Expr.Neq(Val(k), ExprHelper.FunctionCall(nilFunc))));
-
-    ResolveAndTypecheck(options, cmdSeq);
-    return cmdSeq;
-  }
-
-  private List<Cmd> RewriteLheapEmpty(CallCmd callCmd)
-  {
-    GetRelevantInfo(callCmd, out Type type, out Type refType, out Function lheapConstructor,
-      out Function lsetConstructor, out Function lvalConstructor);
-
-    var cmdSeq = new List<Cmd>();
-    var l = callCmd.Outs[0].Decl;
-
-    var mapConstFunc1 = MapConst(refType, Type.Bool);
-    var mapConstFunc2 = MapConst(refType, type);
-
-    cmdSeq.Add(CmdHelper.AssignCmd(l,
-      ExprHelper.FunctionCall(lheapConstructor, ExprHelper.FunctionCall(mapConstFunc1, Expr.False),
-        ExprHelper.FunctionCall(mapConstFunc2, Default(type)))));
-
-    ResolveAndTypecheck(options, cmdSeq);
-    return cmdSeq;
-  }
-
-  private List<Cmd> RewriteLheapAlloc(CallCmd callCmd)
-  {
-    GetRelevantInfo(callCmd, out Type type, out Type refType, out Function lheapConstructor,
-      out Function lsetConstructor, out Function lvalConstructor);
-    var instantiation = monomorphizer.GetTypeInstantiation(callCmd.Proc);
-    var nilFunc = monomorphizer.InstantiateFunction("Nil", instantiation);
-
-    var cmdSeq = new List<Cmd>();
-    var path = callCmd.Ins[0];
-    var v = callCmd.Ins[1];
-    var l = callCmd.Outs[0];
-
-    cmdSeq.Add(CmdHelper.HavocCmd(l));
-    cmdSeq.Add(CmdHelper.AssumeCmd(Expr.Neq(Val(l), ExprHelper.FunctionCall(nilFunc))));
-    cmdSeq.Add(CmdHelper.AssumeCmd(Expr.Not(ExprHelper.FunctionCall(new MapSelect(callCmd.tok, 1), Dom(path), Val(l)))));
-    cmdSeq.Add(CmdHelper.AssumeCmd(Expr.Eq(ExprHelper.FunctionCall(new MapSelect(callCmd.tok, 1), Val(path), Val(l)), v)));
-    cmdSeq.Add(CmdHelper.AssignCmd(
-      CmdHelper.ExprToAssignLhs(path),
-      ExprHelper.FunctionCall(lheapConstructor,
-        ExprHelper.FunctionCall(new MapStore(callCmd.tok, 1), Dom(path), Val(l), Expr.True),
-        Val(path))));
-
-    ResolveAndTypecheck(options, cmdSeq);
-    return cmdSeq;
-  }
-
-  private List<Cmd> RewriteLheapFree(CallCmd callCmd)
-  {
-    GetRelevantInfo(callCmd, out Type type, out Type refType, out Function lheapConstructor,
-      out Function lsetConstructor, out Function lvalConstructor);
-
-    var cmdSeq = new List<Cmd>();
-    var path = callCmd.Ins[0];
-    var k = callCmd.Ins[1];
-
-    var lheapContainsFunc = LheapContains(type);
-    cmdSeq.Add(AssertCmd(callCmd.tok, ExprHelper.FunctionCall(lheapContainsFunc, path, k), "Lheap_Free failed"));
-
-    cmdSeq.Add(
-      CmdHelper.AssignCmd(CmdHelper.ExprToAssignLhs(path),
-      ExprHelper.FunctionCall(lheapConstructor,
-        ExprHelper.FunctionCall(new MapStore(callCmd.tok, 1), Dom(path), k, Expr.False),
-        ExprHelper.FunctionCall(new MapStore(callCmd.tok, 1), Val(path), k, Default(type)))));
-
-    ResolveAndTypecheck(options, cmdSeq);
-    return cmdSeq;
-  }
-
-  private List<Cmd> RewriteLheapGet(CallCmd callCmd)
-  {
-    GetRelevantInfo(callCmd, out Type type, out Type refType, out Function lheapConstructor,
-      out Function lsetConstructor, out Function lvalConstructor);
-
-    var cmdSeq = new List<Cmd>();
-    var path = callCmd.Ins[0];
-    var k = callCmd.Ins[1];
-    var l = callCmd.Outs[0].Decl;
-
-    var mapImpFunc = MapImp(refType);
-    var mapIteFunc = MapIte(refType, type);
-    var mapConstFunc1 = MapConst(refType, Type.Bool);
-    var mapConstFunc2 = MapConst(refType, type);
-    var mapDiffFunc = MapDiff(refType);
-
-    cmdSeq.Add(AssertCmd(callCmd.tok,
-      Expr.Eq(ExprHelper.FunctionCall(mapImpFunc, k, Dom(path)), ExprHelper.FunctionCall(mapConstFunc1, Expr.True)),
-      "Lheap_Get failed"));
-
-    cmdSeq.Add(CmdHelper.AssignCmd(l,
-      ExprHelper.FunctionCall(lheapConstructor, k,
-        ExprHelper.FunctionCall(mapIteFunc, k, Val(path), ExprHelper.FunctionCall(mapConstFunc2, Default(type))))));
-
-    cmdSeq.Add(CmdHelper.AssignCmd(CmdHelper.ExprToAssignLhs(path),
-      ExprHelper.FunctionCall(lheapConstructor, ExprHelper.FunctionCall(mapDiffFunc, Dom(path), k),
-        ExprHelper.FunctionCall(mapIteFunc, ExprHelper.FunctionCall(mapDiffFunc, Dom(path), k), Val(path),
-          ExprHelper.FunctionCall(mapConstFunc2, Default(type))))));
-
-    ResolveAndTypecheck(options, cmdSeq);
-    return cmdSeq;
-  }
-
-  private List<Cmd> RewriteLheapPut(CallCmd callCmd)
-  {
-    GetRelevantInfo(callCmd, out Type type, out Type refType, out Function lheapConstructor,
-      out Function lsetConstructor, out Function lvalConstructor);
-
-    var cmdSeq = new List<Cmd>();
-    var path = callCmd.Ins[0];
-    var l = callCmd.Ins[1];
-
-    var mapOrFunc = MapOr(refType);
-    var mapIteFunc = MapIte(refType, type);
-    cmdSeq.Add(CmdHelper.AssignCmd(
-      CmdHelper.ExprToAssignLhs(path),
-      ExprHelper.FunctionCall(lheapConstructor,
-        ExprHelper.FunctionCall(mapOrFunc, Dom(path), Dom(l)),
-        ExprHelper.FunctionCall(mapIteFunc, Dom(path), Val(path), Val(l)))));
-
-    ResolveAndTypecheck(options, cmdSeq);
-    return cmdSeq;
-  }
-
-  private List<Cmd> RewriteLmapEmpty(CallCmd callCmd)
-  {
-    GetRelevantInfo(callCmd, out Type keyType, out Type valType, out Function lmapConstructor);
-
-    var cmdSeq = new List<Cmd>();
-    var l = callCmd.Outs[0].Decl;
-
-    var mapConstFunc1 = MapConst(keyType, Type.Bool);
-    var mapConstFunc2 = MapConst(keyType, valType);
-
-    cmdSeq.Add(CmdHelper.AssignCmd(l,
-      ExprHelper.FunctionCall(lmapConstructor, ExprHelper.FunctionCall(mapConstFunc1, Expr.False),
-        ExprHelper.FunctionCall(mapConstFunc2, Default(valType)))));
-
-    ResolveAndTypecheck(options, cmdSeq);
-    return cmdSeq;
-  }
-
-  private List<Cmd> RewriteLmapAlloc(CallCmd callCmd)
-  {
-    GetRelevantInfo(callCmd, out Type keyType, out Type valType, out Function lmapConstructor);
-
-    var cmdSeq = new List<Cmd>();
-    var k = callCmd.Ins[0];
-    var val = callCmd.Ins[1];
-    var l = callCmd.Outs[0].Decl;
-
-    var mapIteFunc = MapIte(keyType, valType);
-    var mapConstFunc = MapConst(keyType, valType);
-    cmdSeq.Add(CmdHelper.AssignCmd(l,
-      ExprHelper.FunctionCall(lmapConstructor, Dom(k),
-        ExprHelper.FunctionCall(mapIteFunc, Dom(k), val, ExprHelper.FunctionCall(mapConstFunc, Default(valType))))));
-
-    ResolveAndTypecheck(options, cmdSeq);
-    return cmdSeq;
-  }
-
-  private List<Cmd> RewriteLmapFree(CallCmd callCmd)
-  {
-    GetRelevantInfo(callCmd, out Type keyType, out Type valType, out Function lmapConstructor);
-    var lsetTypeCtorDecl = (DatatypeTypeCtorDecl)monomorphizer.InstantiateTypeCtorDecl("Lset", new List<Type>() { keyType });
-    var lsetConstructor = lsetTypeCtorDecl.Constructors[0];
-
-    var cmdSeq = new List<Cmd>();
-    var l = callCmd.Ins[0];
-    var k = callCmd.Outs[0].Decl;
-
-    cmdSeq.Add(CmdHelper.AssignCmd(k, ExprHelper.FunctionCall(lsetConstructor, Dom(l))));
-
-    ResolveAndTypecheck(options, cmdSeq);
-    return cmdSeq;
-  }
-
-  private List<Cmd> RewriteLmapGet(CallCmd callCmd)
-  {
-    GetRelevantInfo(callCmd, out Type keyType, out Type valType, out Function lmapConstructor);
-
-    var cmdSeq = new List<Cmd>();
-    var path = callCmd.Ins[0];
-    var k = callCmd.Ins[1];
-    var l = callCmd.Outs[0].Decl;
-
-    var mapImpFunc = MapImp(keyType);
-    var mapIteFunc = MapIte(keyType, valType);
-    var mapConstFunc1 = MapConst(keyType, Type.Bool);
-    var mapConstFunc2 = MapConst(keyType, valType);
-    var mapDiffFunc = MapDiff(keyType);
-
-    cmdSeq.Add(AssertCmd(callCmd.tok,
-      Expr.Eq(ExprHelper.FunctionCall(mapImpFunc, k, Dom(path)), ExprHelper.FunctionCall(mapConstFunc1, Expr.True)),
-      "Lmap_Get failed"));
-
-    cmdSeq.Add(CmdHelper.AssignCmd(l,
-      ExprHelper.FunctionCall(lmapConstructor, k,
-        ExprHelper.FunctionCall(mapIteFunc, k, Val(path), ExprHelper.FunctionCall(mapConstFunc2, Default(valType))))));
-
-    cmdSeq.Add(CmdHelper.AssignCmd(CmdHelper.ExprToAssignLhs(path),
-      ExprHelper.FunctionCall(lmapConstructor, ExprHelper.FunctionCall(mapDiffFunc, Dom(path), k),
-        ExprHelper.FunctionCall(mapIteFunc, ExprHelper.FunctionCall(mapDiffFunc, Dom(path), k), Val(path),
-          ExprHelper.FunctionCall(mapConstFunc2, Default(valType))))));
-
-    ResolveAndTypecheck(options, cmdSeq);
-    return cmdSeq;
-  }
-
-  private List<Cmd> RewriteLmapPut(CallCmd callCmd)
-  {
-    GetRelevantInfo(callCmd, out Type keyType, out Type valType, out Function lmapConstructor);
-
-    var cmdSeq = new List<Cmd>();
-    var path = callCmd.Ins[0];
-    var l = callCmd.Ins[1];
-
-    var mapOrFunc = MapOr(keyType);
-    var mapIteFunc = MapIte(keyType, valType);
-    cmdSeq.Add(CmdHelper.AssignCmd(
-      CmdHelper.ExprToAssignLhs(path),
-      ExprHelper.FunctionCall(lmapConstructor,
-        ExprHelper.FunctionCall(mapOrFunc, Dom(path), Dom(l)),
-        ExprHelper.FunctionCall(mapIteFunc, Dom(path), Val(path), Val(l)))));
-
-    ResolveAndTypecheck(options, cmdSeq);
-    return cmdSeq;
-  }
-
   private List<Cmd> RewriteLsetEmpty(CallCmd callCmd)
   {
-    GetRelevantInfo(callCmd, out Type type, out Type refType, out Function lheapConstructor,
+    GetRelevantInfo(callCmd, out Type type, out Type refType,
       out Function lsetConstructor, out Function lvalConstructor);
 
     var cmdSeq = new List<Cmd>();
@@ -439,7 +180,7 @@ public class LinearRewriter
 
   private List<Cmd> RewriteLsetSplit(CallCmd callCmd)
   {
-    GetRelevantInfo(callCmd, out Type type, out Type refType, out Function lheapConstructor,
+    GetRelevantInfo(callCmd, out Type type, out Type refType,
       out Function lsetConstructor, out Function lvalConstructor);
 
     var cmdSeq = new List<Cmd>();
@@ -462,7 +203,7 @@ public class LinearRewriter
 
   private List<Cmd> RewriteLsetGet(CallCmd callCmd)
   {
-    GetRelevantInfo(callCmd, out Type type, out Type refType, out Function lheapConstructor,
+    GetRelevantInfo(callCmd, out Type type, out Type refType,
       out Function lsetConstructor, out Function lvalConstructor);
 
     var cmdSeq = new List<Cmd>();
@@ -488,7 +229,7 @@ public class LinearRewriter
 
   private List<Cmd> RewriteLsetPut(CallCmd callCmd)
   {
-    GetRelevantInfo(callCmd, out Type type, out Type refType, out Function lheapConstructor,
+    GetRelevantInfo(callCmd, out Type type, out Type refType,
       out Function lsetConstructor, out Function lvalConstructor);
 
     var cmdSeq = new List<Cmd>();
@@ -506,7 +247,7 @@ public class LinearRewriter
 
   private List<Cmd> RewriteLvalSplit(CallCmd callCmd)
   {
-    GetRelevantInfo(callCmd, out Type type, out Type refType, out Function lheapConstructor,
+    GetRelevantInfo(callCmd, out Type type, out Type refType,
       out Function lsetConstructor, out Function lvalConstructor);
 
     var cmdSeq = new List<Cmd>();
@@ -528,7 +269,7 @@ public class LinearRewriter
 
   private List<Cmd> RewriteLvalGet(CallCmd callCmd)
   {
-    GetRelevantInfo(callCmd, out Type type, out Type refType, out Function lheapConstructor,
+    GetRelevantInfo(callCmd, out Type type, out Type refType,
       out Function lsetConstructor, out Function lvalConstructor);
 
     var cmdSeq = new List<Cmd>();
@@ -553,7 +294,7 @@ public class LinearRewriter
 
   private List<Cmd> RewriteLvalPut(CallCmd callCmd)
   {
-    GetRelevantInfo(callCmd, out Type type, out Type refType, out Function lheapConstructor,
+    GetRelevantInfo(callCmd, out Type type, out Type refType,
       out Function lsetConstructor, out Function lvalConstructor);
 
     var cmdSeq = new List<Cmd>();
@@ -571,7 +312,7 @@ public class LinearRewriter
     return cmdSeq;
   }
 
-  private void GetRelevantInfo(CallCmd callCmd, out Type type, out Type refType, out Function lheapConstructor,
+  private void GetRelevantInfo(CallCmd callCmd, out Type type, out Type refType,
     out Function lsetConstructor, out Function lvalConstructor)
   {
     var instantiation = monomorphizer.GetTypeInstantiation(callCmd.Proc);
@@ -579,22 +320,10 @@ public class LinearRewriter
     var actualTypeParams = new List<Type>() { type };
     var refTypeCtorDecl = monomorphizer.InstantiateTypeCtorDecl("Ref", actualTypeParams);
     refType = new CtorType(Token.NoToken, refTypeCtorDecl, new List<Type>());
-    var lheapTypeCtorDecl = (DatatypeTypeCtorDecl)monomorphizer.InstantiateTypeCtorDecl("Lheap", actualTypeParams);
-    lheapConstructor = lheapTypeCtorDecl.Constructors[0];
     var lsetTypeCtorDecl = (DatatypeTypeCtorDecl)monomorphizer.InstantiateTypeCtorDecl("Lset", actualTypeParams);
     lsetConstructor = lsetTypeCtorDecl.Constructors[0];
     var lvalTypeCtorDecl = (DatatypeTypeCtorDecl)monomorphizer.InstantiateTypeCtorDecl("Lval", actualTypeParams);
     lvalConstructor = lvalTypeCtorDecl.Constructors[0];
-  }
-
-  private void GetRelevantInfo(CallCmd callCmd, out Type keyType, out Type valType, out Function lmapConstructor)
-  {
-    var instantiation = monomorphizer.GetTypeInstantiation(callCmd.Proc);
-    keyType = instantiation["K"];
-    valType = instantiation["V"];
-    var actualTypeParams = new List<Type>() { keyType, valType };
-    var lmapTypeCtorDecl = (DatatypeTypeCtorDecl)monomorphizer.InstantiateTypeCtorDecl("Lmap", actualTypeParams);
-    lmapConstructor = lmapTypeCtorDecl.Constructors[0];
   }
 
   private void ResolveAndTypecheck(CoreOptions options, IEnumerable<Absy> absys)
@@ -623,14 +352,15 @@ public class LinearRewriter
       if (nAryExpr.Fun is MapSelect)
       {
         var mapExpr = nAryExpr.Args[0];
-        if (mapExpr is NAryExpr lheapValExpr &&
-            lheapValExpr.Fun is FieldAccess &&
-            lheapValExpr.Args[0].Type is CtorType ctorType &&
-            Monomorphizer.GetOriginalDecl(ctorType.Decl).Name == "Lheap")
+        if (mapExpr is NAryExpr mapValExpr &&
+            mapValExpr.Fun is FieldAccess fa &&
+            fa.FieldName == "val" &&
+            mapValExpr.Args[0].Type is CtorType ctorType &&
+            Monomorphizer.GetOriginalDecl(ctorType.Decl).Name == "Map")
         {
-          var cmdSeq = CreateAccessAsserts(lheapValExpr.Args[0], tok, msg);
-          var lheapContainsFunc = LheapContains(nAryExpr.Type);
-          cmdSeq.Add(AssertCmd(tok, ExprHelper.FunctionCall(lheapContainsFunc, lheapValExpr.Args[0], nAryExpr.Args[1]), msg));
+          var cmdSeq = CreateAccessAsserts(mapValExpr.Args[0], tok, msg);
+          var mapContainsFunc = MapContains(nAryExpr.Args[1].Type, nAryExpr.Type);
+          cmdSeq.Add(AssertCmd(tok, ExprHelper.FunctionCall(mapContainsFunc, mapValExpr.Args[0], nAryExpr.Args[1]), msg));
           return cmdSeq;
         }
       }
@@ -646,12 +376,13 @@ public class LinearRewriter
     }
     if (assignLhs is MapAssignLhs mapAssignLhs &&
         mapAssignLhs.Map is FieldAssignLhs fieldAssignLhs1 &&
+        fieldAssignLhs1.FieldAccess.FieldName == "val" &&
         fieldAssignLhs1.Datatype.Type is CtorType ctorType &&
-        Monomorphizer.GetOriginalDecl(ctorType.Decl).Name == "Lheap")
+        Monomorphizer.GetOriginalDecl(ctorType.Decl).Name == "Map")
     {
       var cmdSeq = CreateAccessAsserts(mapAssignLhs.Map, tok, msg);
-      var lheapContainsFunc = LheapContains(mapAssignLhs.Map.Type);
-      cmdSeq.Add(AssertCmd(tok, ExprHelper.FunctionCall(lheapContainsFunc, fieldAssignLhs1.Datatype.AsExpr, mapAssignLhs.Indexes[0]), msg));
+      var mapContainsFunc = MapContains(mapAssignLhs.Indexes[0].Type, mapAssignLhs.Map.Type);
+      cmdSeq.Add(AssertCmd(tok, ExprHelper.FunctionCall(mapContainsFunc, fieldAssignLhs1.Datatype.AsExpr, mapAssignLhs.Indexes[0]), msg));
       return cmdSeq;
     }
     return new List<Cmd>();
